further improvements: syntax, binder modified definition of identity relations

PrincipiaMetaphysicaAutomationPart1/TheoryOfAbstractObjectsV1.thy
@@ -47,7 +47,8 @@ section {* Introduction *}
 
  text {* The encoding of modal functional type theory in functional type theory as explored in 
  previous work \cite{J23,C40} is simple: modal logic formulas are identified with certain functional 
- type theory formulas of predicate type @{text "io"}. Possible worlds are explicitly represented by 
+ type theory formulas of predicate type @{text "i\<Rightarrow>bool"} (abbreviated as @{text "io"} below). 
+ Possible worlds are explicitly represented by 
  terms of type  @{text "i"}. A modal logic @{text "\<phi>"} formula holds for a world @{text "w"} if and 
  only if the application @{text "\<phi> w"} evaluates to true. The definition of the propositional modal logic 
  connectives is then straightforward and it simply realizes the standard translation as a set of equations 
@@ -56,7 +57,7 @@ section {* Introduction *}
  as ordinary logical connectives. No extra binding mechanism is needed since the already existing 
  lambda binding mechanism can be elegantly utilized. 
   
- The challenge in this work is to appropriately 'restrict' this embedding for modal relational type theory.
+ The challenge here is to appropriately 'restrict' this embedding for modal relational type theory.
   \begin{figure}[t]
  \includegraphics[height=5.5cm]{ModalRelationalTypeTheory.png}\includegraphics[height=4.5cm]{ModalRelationalTypeTheory2.png}
  \caption{Grammar of Modal Relational Type Theory. \label{mmrt}
@@ -77,7 +78,7 @@ section {* Introduction *}
 section {* Preliminaries *}
  text {* 
  We start out with some type declarations and type abbreviations. 
- Our formalism explicitly encodes Kripke style semantics. Hence, we introduce a 
+ Our formalism explicitly encodes possible world semantics. Hence, we introduce a 
  distinguished type @{text "i"} to represent the set of possible worlds. 
  Consequently, terms of this type denote possible worlds. 
  Moreover, modal logic formulas are associated in our approach with
@@ -99,8 +100,8 @@ typedecl e
 
  text {*
  To explicitly model the syntactical restrictions of modal relational type theory we introduce a 
- datatype @{text "'a opt"} based on four constructors:
- @{text "ERR 'a"} (identifies erroneous term constructions), @{text "P 'a"} (identifies 
+ (polymorphic) datatype @{text "'a opt"} (where @{text "'a"} is a polymorphic variable in Isabelle) 
+ based on four constructors: @{text "ERR 'a"} (identifies erroneous term constructions), @{text "P 'a"} (identifies 
  propositional formulas), @{text "F 'a"} (identifies  formulas), and @{text "T 'a"} (identifies 
  terms, such as lambda abstractions). The embeddings approach will be suitably adapted below so that 
  for each language expression (in the embedded modal relational type theory) the respective datatype 
@@ -115,10 +116,10 @@ datatype 'a opt = ERR 'a | P 'a | F 'a | T 'a
  four syntactical categories for our language constructs.
  *}
 
-abbreviation mkP::"io\<Rightarrow>io opt" ("_\<^sup>P" 110)  where "\<phi>\<^sup>P \<equiv> P \<phi>" 
-abbreviation mkF::"io\<Rightarrow>io opt" ("_\<^sup>F" 110)  where "\<phi>\<^sup>F \<equiv> F \<phi>" 
-abbreviation mkT::"'a\<Rightarrow>'a opt" ("_\<^sup>T" 110)  where "\<phi>\<^sup>T \<equiv> T \<phi>"
-abbreviation mkE::"'a\<Rightarrow>'a opt" ("_\<^sup>E" 110)  where "\<phi>\<^sup>E \<equiv> ERR \<phi>" 
+abbreviation mkP::"io\<Rightarrow>io opt" ("_\<^sup>P" [109] 110)  where "\<phi>\<^sup>P \<equiv> P \<phi>" 
+abbreviation mkF::"io\<Rightarrow>io opt" ("_\<^sup>F" [109] 110)  where "\<phi>\<^sup>F \<equiv> F \<phi>" 
+abbreviation mkT::"'a\<Rightarrow>'a opt" ("_\<^sup>T" [109] 110)  where "\<phi>\<^sup>T \<equiv> T \<phi>"
+abbreviation mkE::"'a\<Rightarrow>'a opt" ("_\<^sup>E" [109] 110)  where "\<phi>\<^sup>E \<equiv> ERR \<phi>" 
 
  text {* Some language constructs in the theory of abstract types, e.g. the actuality operator  
  @{text "\<A>"} ("it is actually the case that"), refer to a (fixed) given world. To model such a 
@@ -140,8 +141,8 @@ section {* Embedding of Modal Relational Type Theory *}
  @{text "\<phi>"} evaluates @{text "\<phi>"} wrt the fixed given world @{text "cw"}. 
  The compound expression @{text "\<A> \<phi>"} inherits its syntactical category  @{text "F"} (formula) or
  @{text "P"} (propositional formula from @{text "\<phi>"}. If the syntactical catagory of  @{text "\<phi>"} is 
- @{text "E"} (error) or @{text "T"} (term), then the syntactical catagory of @{text "\<A> \<phi>"} 
- is @{text "E"} and a dummy entity of appropriate type is returned. This illustrates the very 
+ @{text "ERR"} (error) or @{text "T"} (term), then the syntactical catagory of @{text "\<A> \<phi>"} 
+ is @{text "ERR"} and a dummy entity of appropriate type is returned. This illustrates the very 
  idea of our explicit structure and constraints and this scheme will repeated below
  for all the other language constructs of modal relational type theory. 
  *}
@@ -151,39 +152,39 @@ abbreviation \<A>::"io opt \<Rightarrow> io opt" where "\<A> \<phi> \<equiv> cas
 
  text {* The Principia Metaphysica distinguishes between encoding and exemplifying, ... say more ...
 
- Encoding @{text "\<kappa>\<^sub>1\<Pi>\<^sup>1"} is noted here as @{text "\<kappa>\<^sub>1\<cdot>\<Pi>\<^sup>1"}. 
+ Encoding @{text "\<kappa>\<^sub>1\<Pi>\<^sup>1"} is noted here as @{text "\<lbrace>\<kappa>\<^sub>1,\<Pi>\<^sup>1\<rbrace>"}. 
  Encoding yields formulas and never propositional formulas. In the embedding encoding 
  is identified with predicate application.
  *}
 
 
-abbreviation Enc::"e opt\<Rightarrow>(e\<Rightarrow>io) opt\<Rightarrow>io opt"(**)("\<lbrace>_,_\<rbrace>")(**) where "\<lbrace>x,\<Phi>\<rbrace> \<equiv> case (x,\<Phi>) of 
+abbreviation Enc::"e opt\<Rightarrow>(e\<Rightarrow>io) opt\<Rightarrow>io opt" (**)("\<lbrace>_,_\<rbrace>")(**) where "\<lbrace>x,\<Phi>\<rbrace> \<equiv> case (x,\<Phi>) of 
     (T(y),T(Q)) \<Rightarrow> F(\<lambda>w.(Q y) w) | _ \<Rightarrow> ERR(dio)"
 
- text {* Exemplifying formulas @{text "\<Pi>\<^sup>1\<kappa>\<^sub>1"} are noted here as @{text "\<Pi>\<^sup>1\<bullet>\<kappa>\<^sub>1"}.  
+ text {* Exemplifying formulas @{text "\<Pi>\<^sup>1\<kappa>\<^sub>1"} are noted here as @{text "\<lparr>\<Pi>\<^sup>1,\<kappa>\<^sub>1\<rparr>"}.  
  Exemplification yields propositional formulas and never formulas. In the embedding exemplification 
  is identified with predicate application, just as encoding.
  *}
 
-abbreviation Exe1::"(e\<Rightarrow>io) opt\<Rightarrow>e opt\<Rightarrow>io opt"(**)("\<lparr>_,_\<rparr>")(**) where "\<lparr>\<Phi>,x\<rparr> \<equiv> case (\<Phi>,x) of 
+abbreviation Exe1::"(e\<Rightarrow>io) opt\<Rightarrow>e opt\<Rightarrow>io opt" (**)("\<lparr>_,_\<rparr>")(**) where "\<lparr>\<Phi>,x\<rparr> \<equiv> case (\<Phi>,x) of 
     (T(Q),T(y)) \<Rightarrow> P(\<lambda>w.(Q y) w) | _ \<Rightarrow> ERR(dio)"
 
  text {* The Principia Metaphysica supports $n$-ary exemplification constructions. For pragmatical 
  reasons we consider here the cases only for $n\leq 3$.
  *}  
 
-abbreviation Exe2::"(e\<Rightarrow>e\<Rightarrow>io) opt\<Rightarrow>e opt\<Rightarrow>e opt\<Rightarrow>io opt"(**)("\<lparr>_,_,_\<rparr>")(**) where "\<lparr>\<Phi>,x1,x2\<rparr> \<equiv> case (\<Phi>,x1,x2) of 
+abbreviation Exe2::"(e\<Rightarrow>e\<Rightarrow>io) opt\<Rightarrow>e opt\<Rightarrow>e opt\<Rightarrow>io opt" (**)("\<lparr>_,_,_\<rparr>")(**) where "\<lparr>\<Phi>,x1,x2\<rparr> \<equiv> case (\<Phi>,x1,x2) of 
     (T(Q),T(y1),T(y2)) \<Rightarrow> P(\<lambda>w.(Q y1 y2) w) | _ \<Rightarrow> ERR(dio)"
-abbreviation Exe3::"(e\<Rightarrow>e\<Rightarrow>e\<Rightarrow>io) opt\<Rightarrow>e opt\<Rightarrow>e opt\<Rightarrow>e opt\<Rightarrow>io opt"(**)("\<lparr>_,_,_,_\<rparr>") (**) where "\<lparr>\<Phi>,x1,x2,x3\<rparr> \<equiv> case (\<Phi>,x1,x2,x3) of 
+abbreviation Exe3::"(e\<Rightarrow>e\<Rightarrow>e\<Rightarrow>io) opt\<Rightarrow>e opt\<Rightarrow>e opt\<Rightarrow>e opt\<Rightarrow>io opt" (**)("\<lparr>_,_,_,_\<rparr>") (**) where "\<lparr>\<Phi>,x1,x2,x3\<rparr> \<equiv> case (\<Phi>,x1,x2,x3) of 
     (T(Q),T(y1),T(y2),T(y3)) \<Rightarrow> P(\<lambda>w.(Q y1 y2 y3) w) | _ \<Rightarrow> ERR(dio)"
 
  text {* Formations with negation and implication are supported for both, formulas  and propositional
  formulas, and their embeddings are straightforward.
  *}  
 
-abbreviation not::"io opt\<Rightarrow>io opt"(**)("\<^bold>\<not>")(**) where "\<^bold>\<not> \<phi> \<equiv> case \<phi> of 
+abbreviation not::"io opt\<Rightarrow>io opt" (**) ("\<^bold>\<not> _" [58] 59)(**) where "\<^bold>\<not> \<phi> \<equiv> case \<phi> of 
     F(\<psi>) \<Rightarrow> F(\<lambda>w.\<not>(\<psi> w)) | P(\<psi>) \<Rightarrow> P(\<lambda>w.\<not>(\<psi> w)) | _ \<Rightarrow> ERR(dio)"  
-abbreviation implies::"io opt\<Rightarrow>io opt\<Rightarrow>io opt"(**)(infixl "\<^bold>\<rightarrow>" 51)(**) where "\<phi> \<^bold>\<rightarrow> \<psi> \<equiv> case (\<phi>,\<psi>) of 
+abbreviation implies::"io opt\<Rightarrow>io opt\<Rightarrow>io opt" (**)(infixl "\<^bold>\<rightarrow>" 51)(**) where "\<phi> \<^bold>\<rightarrow> \<psi> \<equiv> case (\<phi>,\<psi>) of 
     (F(\<alpha>),F(\<beta>)) \<Rightarrow> F(\<lambda>w. \<alpha> w \<longrightarrow> \<beta> w) | (P(\<alpha>),P(\<beta>)) \<Rightarrow> P(\<lambda>w. \<alpha> w \<longrightarrow> \<beta> w) | _ \<Rightarrow> ERR(dio)"  
 
  text {* Also universal quantification @{text "\<^bold>\<forall>(\<lambda>x.\<phi>)"} (first-order and higher-order) is supported 
@@ -193,13 +194,12 @@ abbreviation implies::"io opt\<Rightarrow>io opt\<Rightarrow>io opt"(**)(infixl 
  introduce binder notation @{text "\<^bold>\<forall>x.\<phi>"} as syntactic sugar for @{text "\<^bold>\<forall>(\<lambda>x.\<phi>)"}.
  *}
 
-abbreviation forall::"('a\<Rightarrow>io opt)\<Rightarrow>io opt"(**)("\<^bold>\<forall>")(**) where "\<^bold>\<forall> \<Phi> \<equiv> case (\<Phi> da) of
+abbreviation forall::"('a\<Rightarrow>io opt)\<Rightarrow>io opt" (**)("\<^bold>\<forall>")(**) where "\<^bold>\<forall> \<Phi> \<equiv> case (\<Phi> da) of
     F(\<phi>) \<Rightarrow> F(\<lambda>w.\<forall>x. case (\<Phi> x) of F(\<psi>) \<Rightarrow> \<psi> w) | P(\<phi>) \<Rightarrow> P(\<lambda>w.\<forall>x. case (\<Phi> x) of P(\<psi>) \<Rightarrow> \<psi> w) | _ \<Rightarrow> ERR(dio)"
-abbreviation forallBinder::"('a\<Rightarrow>io opt)\<Rightarrow>io opt" (binder "\<^bold>\<forall>" [9] 9)  where "\<^bold>\<forall> x. \<phi> x \<equiv> \<^bold>\<forall> \<phi>"
+abbreviation forallBinder::"('a\<Rightarrow>io opt)\<Rightarrow>io opt" (binder "\<^bold>\<forall>" [8] 9)  where "\<^bold>\<forall> x. \<phi> x \<equiv> \<^bold>\<forall> \<phi>"
 
 (*<*)
 lemma bla : "(\<^bold>\<forall>x. \<phi> x) = (\<^bold>\<forall>(\<lambda>x. \<phi> x))" by simp
-lemma bla2 : "(\<^bold>\<forall>x. \<phi>) = (\<^bold>\<forall>(\<lambda>x. \<phi>))" nitpick oops
 (*>*)
 
  text {* The modal @{text "\<^bold>\<box>"} operator is introduced here for logic S5. Since in an equivalence class
@@ -209,7 +209,7 @@ lemma bla2 : "(\<^bold>\<forall>x. \<phi>) = (\<^bold>\<forall>(\<lambda>x. \<ph
  are validated by our modeling of @{text "\<^bold>\<box>"}.
  *}
 
-abbreviation box::"io opt\<Rightarrow>io opt"(**)("\<^bold>\<box>")(**) where "\<^bold>\<box>\<phi> \<equiv> case \<phi> of 
+abbreviation box::"io opt\<Rightarrow>io opt" (**)("\<^bold>\<box> _" [62] 63)(**) where "\<^bold>\<box>\<phi> \<equiv> case \<phi> of 
     F(\<psi>) \<Rightarrow> F(\<lambda>w.\<forall>v. \<psi> v) | P(\<psi>) \<Rightarrow> P(\<lambda>w.\<forall>v. \<psi> v) | _ \<Rightarrow> ERR(dio)"  
 
  text {* n-ary lambda abstraction @{text "\<^bold>\<lambda>\<^sup>0,\<^bold>\<lambda>,\<^bold>\<lambda>\<^sup>2\<^sup>,\<^bold>\<lambda>\<^sup>3,..."}, for $n\geq 0$, is supported in the Principia
@@ -217,20 +217,30 @@ abbreviation box::"io opt\<Rightarrow>io opt"(**)("\<^bold>\<box>")(**) where "\
  straightforward: @{text "\<^bold>\<lambda>\<^sup>0"} is mapped to identity and @{text "\<^bold>\<lambda>,\<^bold>\<lambda>\<^sup>2,\<^bold>\<lambda>\<^sup>3,..."} are mapped to n-ary
  lambda abstractions, that is, @{text "\<^bold>\<lambda>(\<lambda>x.\<phi>)"} is mapped to @{text "(\<lambda>x.\<phi>)"} and @{text "\<^bold>\<lambda>\<^sup>2(\<lambda>xy.\<phi>)"} 
  to @{text "(\<lambda>xy.\<phi>)"}.
- For pragmatical reasons we restrict ourselves here to the cases where $n\leq 0$. 
+ For pragmatical reasons we restrict ourselves here to the cases where $n\leq 0$. Binder notation is
+ introduced for @{text "\<^bold>\<lambda>"} (... unfortuntaley, I don't know yet how this can be achieved as well 
+ for @{text "\<^bold>\<lambda>\<^sup>2,\<^bold>\<lambda>\<^sup>3,..."} ...)
  *}
 
-abbreviation lam0::"io opt\<Rightarrow>io opt"(**)("\<^bold>\<lambda>\<^sup>0")(**) where "\<^bold>\<lambda>\<^sup>0\<phi> \<equiv> case \<phi> of 
+abbreviation lam0::"io opt\<Rightarrow>io opt" (**)("\<^bold>\<lambda>\<^sup>0")(**) where "\<^bold>\<lambda>\<^sup>0\<phi> \<equiv> case \<phi> of 
     P(\<psi>) \<Rightarrow> P(\<psi>) | _ \<Rightarrow> ERR dio"  
 
-abbreviation lam::"(e\<Rightarrow>io opt)\<Rightarrow>(e\<Rightarrow>io) opt"(**)("\<^bold>\<lambda>")(**) where "\<^bold>\<lambda>\<Phi> \<equiv> case (\<Phi> de) of
+abbreviation lam::"(e\<Rightarrow>io opt)\<Rightarrow>(e\<Rightarrow>io) opt" (**)("\<^bold>\<lambda>")(**) where "\<^bold>\<lambda>\<Phi> \<equiv> case (\<Phi> de) of
     P(\<phi>) \<Rightarrow> T(\<lambda>x. case (\<Phi> x) of P(\<phi>) \<Rightarrow> \<phi>) | _ \<Rightarrow> ERR(\<lambda>x. dio)"
-abbreviation lam1Binder::"(e\<Rightarrow>io opt)\<Rightarrow>(e\<Rightarrow>io) opt" (binder "\<^bold>\<lambda>" [9] 9)  where "\<^bold>\<lambda> x. \<phi> x \<equiv> \<^bold>\<lambda> \<phi>"
+abbreviation lamBinder::"(e\<Rightarrow>io opt)\<Rightarrow>(e\<Rightarrow>io) opt" (binder "\<^bold>\<lambda>" [8] 9)  where "\<^bold>\<lambda> x. \<phi> x \<equiv> \<^bold>\<lambda> \<phi>"
 
-abbreviation lam2::"(e\<Rightarrow>e\<Rightarrow>io opt)\<Rightarrow>(e\<Rightarrow>e\<Rightarrow>io) opt"(**)("\<^bold>\<lambda>\<^sup>2")(**) where "\<^bold>\<lambda>\<^sup>2\<Phi> \<equiv> case (\<Phi> de de) of
+(*
+abbreviation lamtest::"(e\<Rightarrow>io opt)\<Rightarrow>(e\<Rightarrow>io) opt" (**)("lamm")(**) where "lamm \<Phi> \<equiv> case (\<Phi> de) of
+    P(\<phi>) \<Rightarrow> T(\<lambda>x. case (\<Phi> x) of P(\<phi>) \<Rightarrow> \<phi>) | _ \<Rightarrow> ERR(\<lambda>x. dio)"
+abbreviation lamtestBinder::"(e\<Rightarrow>io opt)\<Rightarrow>(e\<Rightarrow>io) opt" (binder "lam" [8] 9)  where "lam x. \<phi> x \<equiv> lamm \<phi>"
+lemma "(lam x y. \<lparr>R\<^sup>T,x\<^sup>T\<rparr> \<^bold>\<rightarrow> \<lparr>R\<^sup>T,y\<^sup>T\<rparr>) = X" apply simp oops
+lemma "(\<^bold>\<lambda>x y. \<lparr>R\<^sup>T,x\<^sup>T\<rparr> \<^bold>\<rightarrow> \<lparr>R\<^sup>T,y\<^sup>T\<rparr>) = X" apply simp oops
+*)
+
+abbreviation lam2::"(e\<Rightarrow>e\<Rightarrow>io opt)\<Rightarrow>(e\<Rightarrow>e\<Rightarrow>io) opt" (**)("\<^bold>\<lambda>\<^sup>2")(**) where "\<^bold>\<lambda>\<^sup>2\<Phi> \<equiv> case (\<Phi> de de) of
     P(\<phi>) \<Rightarrow> T(\<lambda>x y. case (\<Phi> x y) of P(\<phi>) \<Rightarrow> \<phi>) | _ \<Rightarrow> ERR(\<lambda>x y. dio)"
 
-abbreviation lam3::"(e\<Rightarrow>e\<Rightarrow>e\<Rightarrow>io opt)\<Rightarrow>(e\<Rightarrow>e\<Rightarrow>e\<Rightarrow>io) opt"(**)("\<^bold>\<lambda>\<^sup>3")(**) where "\<^bold>\<lambda>\<^sup>3\<Phi> \<equiv> case (\<Phi> de de de) of
+abbreviation lam3::"(e\<Rightarrow>e\<Rightarrow>e\<Rightarrow>io opt)\<Rightarrow>(e\<Rightarrow>e\<Rightarrow>e\<Rightarrow>io) opt" (**)("\<^bold>\<lambda>\<^sup>3")(**) where "\<^bold>\<lambda>\<^sup>3\<Phi> \<equiv> case (\<Phi> de de de) of
     P(\<phi>) \<Rightarrow> T(\<lambda>x y z. case (\<Phi> x y z) of P(\<phi>) \<Rightarrow> \<phi>) | _ \<Rightarrow> ERR(\<lambda>x y z. dio)"
 
 
@@ -239,11 +249,12 @@ abbreviation lam3::"(e\<Rightarrow>e\<Rightarrow>e\<Rightarrow>io opt)\<Rightarr
  is utilized and evaluation is rigidly carried out with respect to the current world @{text "cw"}.
  Moreover, application of that is allowed only if the body of @{text "\<Phi>"}, computed by clause 
  @{text "(\<Phi> de)"}, is a propositional formula. In this case a term is returned and otherwise error 
- reported (for dummy entity @{text "de"}). 
+ reported (for dummy entity @{text "de"}). We again introduce binder notation.
  *}
  
-abbreviation that::"(e\<Rightarrow>io opt)\<Rightarrow>e opt"(**)("\<iota>")(**)  where "\<iota> \<Phi> \<equiv> case (\<Phi> de) of
+abbreviation that::"(e\<Rightarrow>io opt)\<Rightarrow>e opt" (**)("\<iota>")(**)  where "\<iota> \<Phi> \<equiv> case (\<Phi> de) of
     P(\<phi>) \<Rightarrow> T(THE x. case (\<Phi> x) of P \<psi> \<Rightarrow> \<psi> cw) | _ \<Rightarrow> ERR(de)"
+abbreviation thatBinder::"(e\<Rightarrow>io opt)\<Rightarrow>e opt" (binder "\<iota>" [8] 9)  where "\<iota> x. \<phi> x \<equiv> \<iota> \<phi>"
 
 
 section {* Further Logical Connectives *}
@@ -254,16 +265,16 @@ section {* Further Logical Connectives *}
  to prefer native introductions for all connectives. 
  *}
 
-abbreviation conj::"io opt\<Rightarrow>io opt\<Rightarrow>io opt"(**)(infixl "\<^bold>\<and>" 53)(**) where "\<phi>\<^bold>\<and>\<psi> \<equiv> \<^bold>\<not>(\<phi>\<^bold>\<rightarrow>\<^bold>\<not>\<psi>)"
-abbreviation or::"io opt\<Rightarrow>io opt\<Rightarrow>io opt"(**)(infixl "\<^bold>\<or>" 52)(**) where "\<phi>\<^bold>\<or>\<psi> \<equiv> \<^bold>\<not>\<phi>\<^bold>\<rightarrow>\<psi>"
-abbreviation equivalent::"io opt\<Rightarrow>io opt\<Rightarrow>io opt"(**)(infixl "\<^bold>\<equiv>" 52)(**) where "\<phi>\<^bold>\<equiv>\<psi> \<equiv> (\<phi>\<^bold>\<rightarrow>\<psi>)\<^bold>\<and>(\<psi>\<^bold>\<rightarrow>\<phi>)"
-abbreviation diamond::"io opt\<Rightarrow>io opt"(**)("\<^bold>\<diamond>")(**) where "\<^bold>\<diamond>\<phi> \<equiv> \<^bold>\<not>(\<^bold>\<box>(\<^bold>\<not> \<phi>))"
-abbreviation exists::"('a\<Rightarrow>io opt)\<Rightarrow>io opt"(**)("\<^bold>\<exists>")(**) where "\<^bold>\<exists>\<Phi> \<equiv> case (\<Phi> da) of
+abbreviation conj::"io opt\<Rightarrow>io opt\<Rightarrow>io opt" (**)(infixl "\<^bold>\<and>" 53)(**) where "\<phi>\<^bold>\<and>\<psi> \<equiv> \<^bold>\<not>(\<phi>\<^bold>\<rightarrow>\<^bold>\<not>\<psi>)"
+abbreviation or::"io opt\<Rightarrow>io opt\<Rightarrow>io opt" (**)(infixl "\<^bold>\<or>" 52)(**) where "\<phi>\<^bold>\<or>\<psi> \<equiv> \<^bold>\<not>\<phi>\<^bold>\<rightarrow>\<psi>"
+abbreviation equivalent::"io opt\<Rightarrow>io opt\<Rightarrow>io opt" (**)(infixl "\<^bold>\<equiv>" 51)(**) where "\<phi>\<^bold>\<equiv>\<psi> \<equiv> (\<phi>\<^bold>\<rightarrow>\<psi>)\<^bold>\<and>(\<psi>\<^bold>\<rightarrow>\<phi>)"
+abbreviation diamond::"io opt\<Rightarrow>io opt" (**)("\<^bold>\<diamond> _" [62] 63)(**) where "\<^bold>\<diamond>\<phi> \<equiv> \<^bold>\<not>\<^bold>\<box>(\<^bold>\<not>\<phi>)"
+abbreviation exists::"('a\<Rightarrow>io opt)\<Rightarrow>io opt" (**)("\<^bold>\<exists>")(**) where "\<^bold>\<exists>\<Phi> \<equiv> case (\<Phi> da) of
     P \<phi> \<Rightarrow> P(\<lambda>w.\<exists>x. case (\<Phi> x) of P \<psi> \<Rightarrow> \<psi> w) | F \<phi> \<Rightarrow> F(\<lambda>w. \<exists>x. case (\<Phi> x) of F \<psi> \<Rightarrow> \<psi> w) | _ \<Rightarrow> ERR dio" 
-abbreviation existsBinder::"('a\<Rightarrow>io opt)\<Rightarrow>io opt" (binder "\<^bold>\<exists>" [9] 9)  where "\<^bold>\<exists> x. \<phi> x \<equiv> \<^bold>\<exists> \<phi>"
+abbreviation existsBinder::"('a\<Rightarrow>io opt)\<Rightarrow>io opt" (binder "\<^bold>\<exists>" [8] 9)  where "\<^bold>\<exists> x. \<phi> x \<equiv> \<^bold>\<exists> \<phi>"
 
-(* abbreviation true::"io opt"(**)("\<top>\<^sup>z")(**) where "\<top>\<^sup>z \<equiv> todo; not entirely clear yet " *)
-(* abbreviation alse::"io opt"(**)("\<bottom>\<^sup>z")(**) where "\<bottom>\<^sup>z \<equiv> todo; not entirely clear yet " *)
+(* abbreviation true::"io opt" (**)("\<top>\<^sup>z")(**) where "\<top>\<^sup>z \<equiv> todo; not entirely clear yet " *)
+(* abbreviation alse::"io opt" (**)("\<bottom>\<^sup>z")(**) where "\<bottom>\<^sup>z \<equiv> todo; not entirely clear yet " *)
 
 
 section {* Meta-Logic*}
@@ -315,13 +326,13 @@ text {* Equivalence operator *}
  *}
 
 (*<*) no_syntax "_list" :: "args \<Rightarrow> 'a list" ("[(_)]") (*>*) 
-abbreviation valid :: "io opt\<Rightarrow>mf" (**)("[_]")(**) where "[\<phi>] \<equiv> case \<phi> of 
+abbreviation valid :: "io opt\<Rightarrow>mf" (**)("[_]" [1])(**) where "[\<phi>] \<equiv> case \<phi> of 
     P(\<psi>) \<Rightarrow> if \<forall>w.(\<psi> w) \<longleftrightarrow> True then \<top> else \<bottom> | F(\<psi>) \<Rightarrow> if \<forall>w.(\<psi> w) \<longleftrightarrow> True then \<top> else \<bottom> | _ \<Rightarrow> *"
-abbreviation satisfiable :: "io opt\<Rightarrow>mf" (**)("[_]\<^sup>s\<^sup>a\<^sup>t")(**) where "[\<phi>]\<^sup>s\<^sup>a\<^sup>t \<equiv> case \<phi> of 
+abbreviation satisfiable :: "io opt\<Rightarrow>mf" (**)("[_]\<^sup>s\<^sup>a\<^sup>t" [1])(**) where "[\<phi>]\<^sup>s\<^sup>a\<^sup>t \<equiv> case \<phi> of 
     P(\<psi>) \<Rightarrow> if \<exists>w.(\<psi> w) \<longleftrightarrow> True then \<top> else \<bottom> | F(\<psi>) \<Rightarrow> if \<exists>w.(\<psi> w) \<longleftrightarrow> True then \<top> else \<bottom> | _ \<Rightarrow> *"
-abbreviation countersatisfiable :: "io opt\<Rightarrow>mf" (**)("[_]\<^sup>c\<^sup>s\<^sup>a\<^sup>t")(**) where "[\<phi>]\<^sup>c\<^sup>s\<^sup>a\<^sup>t \<equiv>  case \<phi> of 
+abbreviation countersatisfiable :: "io opt\<Rightarrow>mf" (**)("[_]\<^sup>c\<^sup>s\<^sup>a\<^sup>t" [1])(**) where "[\<phi>]\<^sup>c\<^sup>s\<^sup>a\<^sup>t \<equiv>  case \<phi> of 
     P(\<psi>) \<Rightarrow> if \<exists>w.\<not>(\<psi> w) \<longleftrightarrow> True then \<top> else \<bottom> | F(\<psi>) \<Rightarrow> if \<exists>w.\<not>(\<psi> w) \<longleftrightarrow> True then \<top> else \<bottom> | _ \<Rightarrow> *"
-abbreviation invalid :: "io opt\<Rightarrow>mf" (**)("[_]\<^sup>i\<^sup>n\<^sup>v")(**) where "[\<phi>]\<^sup>i\<^sup>n\<^sup>v \<equiv> case \<phi> of 
+abbreviation invalid :: "io opt\<Rightarrow>mf" (**)("[_]\<^sup>i\<^sup>n\<^sup>v" [1])(**) where "[\<phi>]\<^sup>i\<^sup>n\<^sup>v \<equiv> case \<phi> of 
     P(\<psi>) \<Rightarrow> if \<forall>w.\<not>(\<psi> w) \<longleftrightarrow> True then \<top> else \<bottom> | F(\<psi>) \<Rightarrow> if \<forall>w.\<not>(\<psi> w) \<longleftrightarrow> True then \<top> else \<bottom> | _ \<Rightarrow> *"
 
 
@@ -333,61 +344,61 @@ section {* Some Basic Tests *}
  and arbitrary propositional formulas. We present the lemma in both variants. 
  *}
  
-lemma necessitationF: "[\<phi>\<^sup>F] = \<top> \<longrightarrow> [\<^bold>\<box>(\<phi>\<^sup>F)] = \<top>" apply simp done
-lemma necessitationP: "[\<phi>\<^sup>P] = \<top> \<longrightarrow> [\<^bold>\<box>(\<phi>\<^sup>P)] = \<top>" apply simp done
+lemma necessitationF: "[\<phi>\<^sup>F] = \<top> \<longrightarrow> [\<^bold>\<box>\<phi>\<^sup>F] = \<top>" apply simp done
+lemma necessitationP: "[\<phi>\<^sup>P] = \<top> \<longrightarrow> [\<^bold>\<box>\<phi>\<^sup>P] = \<top>" apply simp done
 
  subsection {* Modal Collapse is Countersatisfiable *}
 
   text {* The modelfinder Nitpick constructs a finite countermodel to the assertion
   that modal collaps is valid. Nitpicks countermodel consists of four worlds i1, i2, i3 and i4.
   Moreover, it defines  @{text "\<phi>"} to hold only in world i3 and it suggests i3 as the actual 
-  world in which to evaluate the conjecture formula. This countermodel is clearly not minimal.
+  world in which to evaluate the conjecture formula. This countermodel is not minimal.
   *}
 
-lemma modalCollapseF: "[\<phi>\<^sup>F \<^bold>\<rightarrow> \<^bold>\<box>(\<phi>\<^sup>F)] = \<top>" apply simp nitpick oops -- {* Countermodel by Nitpick *}
-lemma modalCollapseP: "[\<phi>\<^sup>P \<^bold>\<rightarrow> \<^bold>\<box>(\<phi>\<^sup>P)] = \<top>" apply simp nitpick oops -- {* Countermodel by Nitpick *}
+lemma modalCollapseF: "[\<phi>\<^sup>F \<^bold>\<rightarrow> \<^bold>\<box>\<phi>\<^sup>F] = \<top>" apply simp nitpick oops -- {* Countermodel by Nitpick *}
+lemma modalCollapseP: "[\<phi>\<^sup>P \<^bold>\<rightarrow> \<^bold>\<box>\<phi>\<^sup>P] = \<top>" apply simp nitpick oops -- {* Countermodel by Nitpick *}
 
 (*
 lemma modalCollapseFcsa: "[\<phi>\<^sup>F \<^bold>\<rightarrow> \<phi>\<^sup>F] = \<top>" sledgehammer [remote_leo2 remote_satallax]
-lemma modalCollapseFcsa: "[\<phi>\<^sup>F \<^bold>\<rightarrow> \<^bold>\<box>(\<phi>\<^sup>F)]\<^sup>c\<^sup>s\<^sup>a\<^sup>t = \<top>" sledgehammer [remote_leo2 remote_satallax]
-lemma modalCollapsePcsa: "[\<phi>\<^sup>P \<^bold>\<rightarrow> \<^bold>\<box>(\<phi>\<^sup>P)]\<^sup>c\<^sup>s\<^sup>a\<^sup>t = \<top>" sledgehammer [remote_leo2 remote_satallax]
+lemma modalCollapseFcsa: "[\<phi>\<^sup>F \<^bold>\<rightarrow> \<^bold>\<box>\<phi>\<^sup>F]\<^sup>c\<^sup>s\<^sup>a\<^sup>t = \<top>" sledgehammer [remote_leo2 remote_satallax]
+lemma modalCollapsePcsa: "[\<phi>\<^sup>P \<^bold>\<rightarrow> \<^bold>\<box>\<phi>\<^sup>P]\<^sup>c\<^sup>s\<^sup>a\<^sup>t = \<top>" sledgehammer [remote_leo2 remote_satallax]
 *)
 
  subsection {* Verifying S5 Principles \label{sec:S5} *} 
 
  text {* @{text "\<box>"} could have been modeled by employing an equivalence relation @{text "r"} in a 
- guarding clause. This has been done in previous work. In a simpler, alternative approach we omitted 
+ guarding clause. This has been done in previous work. In a simpler, alternative approach we omit 
  this clause here (since all worlds are reachable from any world in an equivalence relation). The 
  following lemmata, which check various conditions for S5,  ensure that we have indeed 
- modeled S5 correctly.
+ obtain a correct modeling of S5.
  *}
 
-lemma axiom_T_P: "[\<^bold>\<box>(\<phi>\<^sup>P) \<^bold>\<rightarrow> (\<phi>\<^sup>P)] = \<top>" apply simp done
-lemma axiom_T_F: "[\<^bold>\<box>(\<phi>\<^sup>F) \<^bold>\<rightarrow> (\<phi>\<^sup>F)] = \<top>" apply simp done
+lemma axiom_T_P: "[\<^bold>\<box>\<phi>\<^sup>P \<^bold>\<rightarrow> \<phi>\<^sup>P] = \<top>" apply simp done
+lemma axiom_T_F: "[\<^bold>\<box>\<phi>\<^sup>F \<^bold>\<rightarrow> \<phi>\<^sup>F] = \<top>" apply simp done
 
-lemma axiom_B_P: "[\<phi>\<^sup>P \<^bold>\<rightarrow> \<^bold>\<box>(\<^bold>\<diamond>(\<phi>\<^sup>P))] = \<top>" apply simp done
-lemma axiom_B_F: "[\<phi>\<^sup>F \<^bold>\<rightarrow> \<^bold>\<box>(\<^bold>\<diamond>(\<phi>\<^sup>F))] = \<top>" apply simp done
+lemma axiom_B_P: "[\<phi>\<^sup>P \<^bold>\<rightarrow> \<^bold>\<box>\<^bold>\<diamond>\<phi>\<^sup>P] = \<top>" apply simp done
+lemma axiom_B_F: "[\<phi>\<^sup>F \<^bold>\<rightarrow> \<^bold>\<box>\<^bold>\<diamond>\<phi>\<^sup>F] = \<top>" apply simp done
 
-lemma axiom_4_P: "[\<^bold>\<box>(\<phi>\<^sup>P) \<^bold>\<rightarrow> \<^bold>\<diamond>(\<phi>\<^sup>P)] = \<top>" apply simp by auto
-lemma axiom_4_F: "[\<^bold>\<box>(\<phi>\<^sup>F) \<^bold>\<rightarrow> \<^bold>\<diamond>(\<phi>\<^sup>F)] = \<top>" apply simp by auto
+lemma axiom_4_P: "[\<^bold>\<box>\<phi>\<^sup>P \<^bold>\<rightarrow> \<^bold>\<diamond>\<phi>\<^sup>P] = \<top>" apply simp by auto
+lemma axiom_4_F: "[\<^bold>\<box>\<phi>\<^sup>F \<^bold>\<rightarrow> \<^bold>\<diamond>\<phi>\<^sup>F] = \<top>" apply simp by auto
 
-lemma axiom_D_P: "[\<^bold>\<box>(\<phi>\<^sup>P) \<^bold>\<rightarrow> \<^bold>\<box>(\<^bold>\<box>(\<phi>\<^sup>P))] = \<top>" apply simp done
-lemma axiom_D_F: "[\<^bold>\<box>(\<phi>\<^sup>F) \<^bold>\<rightarrow> \<^bold>\<box>(\<^bold>\<box>(\<phi>\<^sup>F))] = \<top>" apply simp done
+lemma axiom_D_P: "[\<^bold>\<box>\<phi>\<^sup>P \<^bold>\<rightarrow> \<^bold>\<box>\<^bold>\<box>\<phi>\<^sup>P] = \<top>" apply simp done
+lemma axiom_D_F: "[\<^bold>\<box>\<phi>\<^sup>F \<^bold>\<rightarrow> \<^bold>\<box>\<^bold>\<box>\<phi>\<^sup>F] = \<top>" apply simp done
 
-lemma axiom_5_P: "[\<^bold>\<diamond>(\<phi>\<^sup>P) \<^bold>\<rightarrow> \<^bold>\<box>(\<^bold>\<diamond>(\<phi>\<^sup>P))] = \<top>" apply simp done
-lemma axiom_5_F: "[\<^bold>\<diamond>(\<phi>\<^sup>F) \<^bold>\<rightarrow> \<^bold>\<box>(\<^bold>\<diamond>(\<phi>\<^sup>F))] = \<top>" apply simp done
+lemma axiom_5_P: "[\<^bold>\<diamond>\<phi>\<^sup>P \<^bold>\<rightarrow> \<^bold>\<box>\<^bold>\<diamond>\<phi>\<^sup>P] = \<top>" apply simp done
+lemma axiom_5_F: "[\<^bold>\<diamond>\<phi>\<^sup>F \<^bold>\<rightarrow> \<^bold>\<box>\<^bold>\<diamond>\<phi>\<^sup>F] = \<top>" apply simp done
 
-lemma test_A_P: "[\<^bold>\<box>(\<^bold>\<diamond>(\<phi>\<^sup>P)) \<^bold>\<rightarrow> \<^bold>\<diamond>(\<phi>\<^sup>P)] = \<top>" apply simp done
-lemma test_A_F: "[\<^bold>\<box>(\<^bold>\<diamond>(\<phi>\<^sup>F)) \<^bold>\<rightarrow> \<^bold>\<diamond>(\<phi>\<^sup>F)] = \<top>" apply simp done
+lemma test_A_P: "[\<^bold>\<box>\<^bold>\<diamond>\<phi>\<^sup>P \<^bold>\<rightarrow> \<^bold>\<diamond>\<phi>\<^sup>P] = \<top>" apply simp done
+lemma test_A_F: "[\<^bold>\<box>\<^bold>\<diamond>\<phi>\<^sup>F \<^bold>\<rightarrow> \<^bold>\<diamond>\<phi>\<^sup>F] = \<top>" apply simp done
 
-lemma test_B_P: "[\<^bold>\<diamond>(\<^bold>\<box>(\<phi>\<^sup>P)) \<^bold>\<rightarrow> \<^bold>\<diamond>(\<phi>\<^sup>P)] = \<top>" apply simp by auto
-lemma test_B_F: "[\<^bold>\<diamond>(\<^bold>\<box>(\<phi>\<^sup>F)) \<^bold>\<rightarrow> \<^bold>\<diamond>(\<phi>\<^sup>F)] = \<top>" apply simp by auto
+lemma test_B_P: "[\<^bold>\<diamond>\<^bold>\<box>\<phi>\<^sup>P \<^bold>\<rightarrow> \<^bold>\<diamond>\<phi>\<^sup>P] = \<top>" apply simp by auto
+lemma test_B_F: "[\<^bold>\<diamond>\<^bold>\<box>\<phi>\<^sup>F \<^bold>\<rightarrow> \<^bold>\<diamond>\<phi>\<^sup>F] = \<top>" apply simp by auto
 
-lemma test_C_P: "[\<^bold>\<box>(\<^bold>\<diamond>(\<phi>\<^sup>P)) \<^bold>\<rightarrow> \<^bold>\<box>(\<phi>\<^sup>P)] = \<top>" apply simp nitpick oops -- {* Countermodel by Nitpick *}
-lemma test_C_F: "[\<^bold>\<box>(\<^bold>\<diamond>(\<phi>\<^sup>F)) \<^bold>\<rightarrow> \<^bold>\<box>(\<phi>\<^sup>F)] = \<top>" apply simp nitpick oops -- {* Countermodel by Nitpick *}
+lemma test_C_P: "[\<^bold>\<box>\<^bold>\<diamond>\<phi>\<^sup>P \<^bold>\<rightarrow> \<^bold>\<box>\<phi>\<^sup>P] = \<top>" apply simp nitpick oops -- {* Countermodel by Nitpick *}
+lemma test_C_F: "[\<^bold>\<box>\<^bold>\<diamond>\<phi>\<^sup>F \<^bold>\<rightarrow> \<^bold>\<box>\<phi>\<^sup>F] = \<top>" apply simp nitpick oops -- {* Countermodel by Nitpick *}
 
-lemma test_D_P: "[\<^bold>\<diamond>(\<^bold>\<box>(\<phi>\<^sup>P)) \<^bold>\<rightarrow> \<^bold>\<box>(\<phi>\<^sup>P)] = \<top>" apply simp done
-lemma test_D_F: "[\<^bold>\<diamond>(\<^bold>\<box>(\<phi>\<^sup>F)) \<^bold>\<rightarrow> \<^bold>\<box>(\<phi>\<^sup>F)] = \<top>" apply simp done
+lemma test_D_P: "[\<^bold>\<diamond>\<^bold>\<box>\<phi>\<^sup>P \<^bold>\<rightarrow> \<^bold>\<box>\<phi>\<^sup>P] = \<top>" apply simp done
+lemma test_D_F: "[\<^bold>\<diamond>\<^bold>\<box>\<phi>\<^sup>F \<^bold>\<rightarrow> \<^bold>\<box>\<phi>\<^sup>F] = \<top>" apply simp done
 
 
 subsection {* Relations between  Meta-Logical Notions *}
@@ -406,8 +417,8 @@ lemma  "[\<phi>\<^sup>T]\<^sup>i\<^sup>n\<^sup>v = *" apply simp done
 
  subsection {* Testing for the Correct Propagation of Syntactical Category Information *}
 
-lemma "\<exists>X. \<lparr>R\<^sup>T,a\<^sup>T\<rparr> = (X\<^sup>P) \<and> \<not>(\<exists>X. \<lparr>R\<^sup>T,a\<^sup>T\<rparr> = (X\<^sup>F)) \<and> \<not>(\<exists>X. \<lparr>R\<^sup>T,a\<^sup>T\<rparr> = (X\<^sup>T)) \<and> \<not>(\<exists>X. \<lparr>R\<^sup>T,a\<^sup>T\<rparr> = (X\<^sup>E))" apply simp done
-lemma "\<exists>X. \<lbrace>x\<^sup>T,R\<^sup>T\<rbrace> = (X\<^sup>F) \<and> \<not>(\<exists>X. \<lbrace>x\<^sup>T,R\<^sup>T\<rbrace> = (X\<^sup>P)) \<and> \<not>(\<exists>X. \<lbrace>x\<^sup>T,R\<^sup>T\<rbrace> = (X\<^sup>T)) \<and> \<not>(\<exists>X. \<lbrace>x\<^sup>T,R\<^sup>T\<rbrace> = (X\<^sup>E))" apply simp done
+lemma "\<exists>X. \<lparr>R\<^sup>T,a\<^sup>T\<rparr> = X\<^sup>P \<and> \<not>(\<exists>X. \<lparr>R\<^sup>T,a\<^sup>T\<rparr> = X\<^sup>F) \<and> \<not>(\<exists>X. \<lparr>R\<^sup>T,a\<^sup>T\<rparr> = X\<^sup>T) \<and> \<not>(\<exists>X. \<lparr>R\<^sup>T,a\<^sup>T\<rparr> = X\<^sup>E)" apply simp done
+lemma "\<exists>X. \<lbrace>x\<^sup>T,R\<^sup>T\<rbrace> = X\<^sup>F \<and> \<not>(\<exists>X. \<lbrace>x\<^sup>T,R\<^sup>T\<rbrace> = X\<^sup>P) \<and> \<not>(\<exists>X. \<lbrace>x\<^sup>T,R\<^sup>T\<rbrace> = X\<^sup>T) \<and> \<not>(\<exists>X. \<lbrace>x\<^sup>T,R\<^sup>T\<rbrace> = X\<^sup>E)" apply simp done
 
  text {* Most importantly, we have that the following language constructing is evaluated as erroneous at validity
  level. *}
@@ -423,10 +434,10 @@ lemma "[\<lparr>\<^bold>\<lambda>x. \<lparr>R\<^sup>T,x\<^sup>T\<rparr> \<^bold>
 
 lemma "\<lparr>\<^bold>\<lambda>x. \<lparr>R\<^sup>T,x\<^sup>T\<rparr> \<^bold>\<rightarrow> \<lbrace>x\<^sup>T,R\<^sup>T\<rbrace>,a\<^sup>T\<rparr> = X" apply simp oops
 
-lemma "\<exists>X. \<lparr>\<^bold>\<lambda>x. \<lparr>R\<^sup>T,x\<^sup>T\<rparr> \<^bold>\<rightarrow> \<lparr>R\<^sup>T,x\<^sup>T\<rparr>,a\<^sup>T\<rparr> = (X\<^sup>P)" apply simp done -- {* Solution: @{text "(\<lambda>w. True) = X"} *}
+lemma "\<exists>X. \<lparr>\<^bold>\<lambda>x. \<lparr>R\<^sup>T,x\<^sup>T\<rparr> \<^bold>\<rightarrow> \<lparr>R\<^sup>T,x\<^sup>T\<rparr>,a\<^sup>T\<rparr> = X\<^sup>P" apply simp done -- {* Solution: @{text "(\<lambda>w. True) = X"} *}
 lemma "[\<lparr>\<^bold>\<lambda>x. \<lparr>R\<^sup>T,x\<^sup>T\<rparr> \<^bold>\<rightarrow> \<lparr>R\<^sup>T,x\<^sup>T\<rparr>,a\<^sup>T\<rparr>] = \<top>" apply simp done
 
-lemma "\<lparr>\<^bold>\<lambda>x. \<lparr>R\<^sup>T,x\<^sup>T\<rparr> \<^bold>\<rightarrow> \<lparr>R\<^sup>T,x\<^sup>T\<rparr>,a\<^sup>T\<rparr> = (X\<^sup>P)" apply simp oops
+lemma "\<lparr>\<^bold>\<lambda>x. \<lparr>R\<^sup>T,x\<^sup>T\<rparr> \<^bold>\<rightarrow> \<lparr>R\<^sup>T,x\<^sup>T\<rparr>,a\<^sup>T\<rparr> = X\<^sup>P" apply simp oops
 lemma "(\<^bold>\<lambda>x. \<lparr>R\<^sup>T,x\<^sup>T\<rparr> \<^bold>\<rightarrow> \<lbrace>x\<^sup>T,R\<^sup>T\<rbrace>) = X" apply simp oops
 
 lemma "[(\<^bold>\<forall>x. \<lparr>R\<^sup>T,x\<^sup>T\<rparr> \<^bold>\<rightarrow> \<lparr>R\<^sup>T,x\<^sup>T\<rparr>)] = \<top>" apply simp done
@@ -438,20 +449,24 @@ lemma "(\<^bold>\<forall>x. \<lbrace>x\<^sup>T,R\<^sup>T\<rbrace> \<^bold>\<righ
 
 lemma "[(\<^bold>\<exists>x y. \<lbrace>x\<^sup>T,R\<^sup>T\<rbrace> \<^bold>\<rightarrow> \<lbrace>y\<^sup>T,R\<^sup>T\<rbrace>)] = \<top>" apply simp done
 
+
 lemma "[(\<^bold>\<forall>x. \<lparr>R\<^sup>T,x\<^sup>T\<rparr> \<^bold>\<rightarrow> \<lbrace>x\<^sup>T,R\<^sup>T\<rbrace>)] = *" apply simp done
 lemma "[(\<^bold>\<forall>x. \<lparr>R\<^sup>T,x\<^sup>T\<rparr> \<^bold>\<rightarrow> \<lbrace>x\<^sup>T,R\<^sup>T\<rbrace>)] = X" apply simp oops
 lemma "(\<^bold>\<forall>x. \<lparr>R\<^sup>T,x\<^sup>T\<rparr> \<^bold>\<rightarrow> \<lbrace>x\<^sup>T,R\<^sup>T\<rbrace>) = X" apply simp oops
 lemma "[(\<^bold>\<forall>R. \<lparr>R\<^sup>T,x\<^sup>T\<rparr> \<^bold>\<rightarrow> \<lbrace>x\<^sup>T,R\<^sup>T\<rbrace>)] = *" apply simp done
 lemma "(\<^bold>\<forall>R. \<lparr>R\<^sup>T,x\<^sup>T\<rparr> \<^bold>\<rightarrow> \<lbrace>x\<^sup>T,R\<^sup>T\<rbrace>) = X" apply simp oops
 
+lemma "[(\<^bold>\<forall>x. \<^bold>\<exists>(\<lambda>R. \<lbrace>x\<^sup>T,R\<^sup>T\<rbrace> \<^bold>\<rightarrow> \<lbrace>x\<^sup>T,R\<^sup>T\<rbrace>))] = \<top>" apply simp done
+lemma "[(\<^bold>\<exists>x. \<^bold>\<forall>(\<lambda>R. \<lbrace>x\<^sup>T,R\<^sup>T\<rbrace> \<^bold>\<rightarrow> \<lbrace>x\<^sup>T,R\<^sup>T\<rbrace>))] = \<top>" apply simp done
+
 
  subsection {* Are Priorities Defined Correctly? *}
 
-lemma "(\<phi>\<^sup>P) \<^bold>\<and> (\<psi>\<^sup>P) \<^bold>\<rightarrow> (\<chi>\<^sup>P) \<equiv> ((\<phi>\<^sup>P) \<^bold>\<and> (\<psi>\<^sup>P)) \<^bold>\<rightarrow> (\<chi>\<^sup>P)" apply simp done
-lemma "(\<phi>\<^sup>P) \<^bold>\<and> (\<psi>\<^sup>P) \<^bold>\<rightarrow> (\<chi>\<^sup>P) \<equiv> (\<phi>\<^sup>P) \<^bold>\<and> ((\<psi>\<^sup>P) \<^bold>\<rightarrow> (\<chi>\<^sup>P))" apply simp nitpick oops -- {* Countermodel by Nitpick *}
+lemma "\<phi>\<^sup>P \<^bold>\<and> \<psi>\<^sup>P \<^bold>\<rightarrow> \<chi>\<^sup>P \<equiv> (\<phi>\<^sup>P \<^bold>\<and> \<psi>\<^sup>P) \<^bold>\<rightarrow> \<chi>\<^sup>P" apply simp done
+lemma "\<phi>\<^sup>P \<^bold>\<and> \<psi>\<^sup>P \<^bold>\<rightarrow> \<chi>\<^sup>P \<equiv> \<phi>\<^sup>P \<^bold>\<and> (\<psi>\<^sup>P \<^bold>\<rightarrow> \<chi>\<^sup>P)" apply simp nitpick oops -- {* Countermodel by Nitpick *}
 
-lemma "((\<phi>\<^sup>P) \<^bold>\<and> (\<psi>\<^sup>P) \<^bold>\<equiv> (\<phi>\<^sup>P) \<^bold>\<and> (\<psi>\<^sup>P)) \<equiv> (((\<phi>\<^sup>P) \<^bold>\<and> (\<psi>\<^sup>P)) \<^bold>\<equiv> ((\<phi>\<^sup>P) \<^bold>\<and> (\<psi>\<^sup>P)))" apply simp done
-lemma "((\<phi>\<^sup>P) \<^bold>\<and> (\<psi>\<^sup>P) \<^bold>\<equiv> (\<phi>\<^sup>P) \<^bold>\<and> (\<psi>\<^sup>P)) \<equiv> ((\<phi>\<^sup>P) \<^bold>\<and> ((\<psi>\<^sup>P) \<^bold>\<equiv> (\<phi>\<^sup>P)) \<^bold>\<and> (\<psi>\<^sup>P))" apply simp nitpick oops -- {* Countermodel by Nitpick *}
+lemma "(\<phi>\<^sup>P \<^bold>\<and> \<psi>\<^sup>P \<^bold>\<equiv> \<phi>\<^sup>P \<^bold>\<and> \<psi>\<^sup>P) \<equiv> ((\<phi>\<^sup>P \<^bold>\<and> \<psi>\<^sup>P) \<^bold>\<equiv> (\<phi>\<^sup>P \<^bold>\<and> \<psi>\<^sup>P))" apply simp done
+lemma "(\<phi>\<^sup>P \<^bold>\<and> \<psi>\<^sup>P \<^bold>\<equiv> \<phi>\<^sup>P \<^bold>\<and> \<psi>\<^sup>P) \<equiv> (\<phi>\<^sup>P \<^bold>\<and> (\<psi>\<^sup>P \<^bold>\<equiv> \<phi>\<^sup>P) \<^bold>\<and> \<psi>\<^sup>P)" apply simp nitpick oops -- {* Countermodel by Nitpick *}
 
 
 section {* E!, O!, A! and =E *}
@@ -462,52 +477,55 @@ consts E::"(e\<Rightarrow>io)"
  
  text {* Being ordinary is defined as being possibly concrete. *}
 
-abbreviation ordinaryObject::"(e\<Rightarrow>io) opt"(**)("O!")(**) where "O! \<equiv> \<^bold>\<lambda>x. \<^bold>\<diamond>\<lparr>E\<^sup>T,x\<^sup>T\<rparr>"
+abbreviation ordinaryObject::"(e\<Rightarrow>io) opt" (**)("O!")(**) where "O! \<equiv> \<^bold>\<lambda>x. \<^bold>\<diamond>\<lparr>E\<^sup>T,x\<^sup>T\<rparr>"
 
  text {* Being abstract is is defined as not possibly being concrete. *}
 
-abbreviation abstractObject::"(e\<Rightarrow>io) opt"(**)("A!")(**) where "A! \<equiv> \<^bold>\<lambda>x. \<^bold>\<not>(\<^bold>\<diamond>\<lparr>E\<^sup>T,x\<^sup>T\<rparr>)"
+abbreviation abstractObject::"(e\<Rightarrow>io) opt" (**)("A!")(**) where "A! \<equiv> \<^bold>\<lambda>x. \<^bold>\<not>(\<^bold>\<diamond>\<lparr>E\<^sup>T,x\<^sup>T\<rparr>)"
 
- text {* Identity @{text "=\<^sub>e"} is defined as .... Subsequenty, the infix operator @{text "=\<^sub>E"} is 
- introduced. 
+ text {* Identity relations @{text "\<^bold>=\<^sub>E"} and @{text "\<^bold>="} are introduced. 
  *}
 
-abbreviation identity::"(e\<Rightarrow>e\<Rightarrow>io) opt"(**)("\<^bold>=\<^sub>e")(**) where "\<^bold>=\<^sub>e \<equiv> 
-  \<^bold>\<lambda>\<^sup>2(\<lambda>x y. (\<lparr>O!,x\<^sup>T\<rparr> \<^bold>\<and> \<lparr>O!,y\<^sup>T\<rparr>) \<^bold>\<and> \<^bold>\<box>(\<^bold>\<forall>(\<lambda>F. \<lparr>F\<^sup>T,x\<^sup>T\<rparr> \<^bold>\<equiv> \<lparr>F\<^sup>T,y\<^sup>T\<rparr>)))"
+(* 
+abbreviation identitye::"(e\<Rightarrow>e\<Rightarrow>io) opt" (**)("\<^bold>=\<^sub>e")(**) where "\<^bold>=\<^sub>e \<equiv> 
+  \<^bold>\<lambda>\<^sup>2(\<lambda>x y. \<lparr>O!,x\<^sup>T\<rparr> \<^bold>\<and> \<lparr>O!,y\<^sup>T\<rparr> \<^bold>\<and> \<^bold>\<box>(\<^bold>\<forall>F. \<lparr>F\<^sup>T,x\<^sup>T\<rparr> \<^bold>\<equiv> \<lparr>F\<^sup>T,y\<^sup>T\<rparr>))"
+abbreviation identityE::"e opt\<Rightarrow>e opt\<Rightarrow>io opt" (**)(infixl "\<^bold>=\<^sub>E" 63)(**) where "x \<^bold>=\<^sub>E y \<equiv> \<lparr>\<^bold>=\<^sub>e,x,y\<rparr>"
+*)
 
-abbreviation identityE::"e opt\<Rightarrow>e opt\<Rightarrow>io opt"(**)(infixl "\<^bold>=\<^sub>E" 63)(**) where "x \<^bold>=\<^sub>E y \<equiv> \<lparr>\<^bold>=\<^sub>e,x,y\<rparr>"
+abbreviation identityE::"e opt\<Rightarrow>e opt\<Rightarrow>io opt" (**)(infixl "\<^bold>=\<^sub>E" 63)(**) 
+  where "x \<^bold>=\<^sub>E y \<equiv> \<lparr>O!,x\<rparr> \<^bold>\<and> \<lparr>O!,y\<rparr> \<^bold>\<and> \<^bold>\<box>(\<^bold>\<forall>F. \<lparr>F\<^sup>T,x\<rparr> \<^bold>\<equiv> \<lparr>F\<^sup>T,y\<rparr>)"
+
+abbreviation identity::"e opt\<Rightarrow>e opt\<Rightarrow>io opt" (**)(infixl "\<^bold>=" 63)(**) 
+  where "x \<^bold>= y \<equiv> (x \<^bold>=\<^sub>E y) \<^bold>\<or> (\<lparr>A!,x\<rparr> \<^bold>\<and> \<lparr>A!,y\<rparr> \<^bold>\<and> \<^bold>\<box>(\<^bold>\<forall>F. \<lbrace>x,F\<^sup>T\<rbrace> \<^bold>\<equiv> \<lbrace>y,F\<^sup>T\<rbrace>))"
 
 
-section {* Further Test Examples *}
+subsection {* Further Test Examples *}
 
  text {* Todo: ... select, adapt, and explain some of examples below *}
 
-lemma "[(\<^bold>\<forall>x. \<^bold>\<exists>(\<lambda>R. \<lbrace>x\<^sup>T,R\<^sup>T\<rbrace> \<^bold>\<rightarrow> \<lbrace>x\<^sup>T,R\<^sup>T\<rbrace>))] = \<top>" apply simp done
-lemma "[(\<^bold>\<exists>x. \<^bold>\<forall>(\<lambda>R. \<lbrace>x\<^sup>T,R\<^sup>T\<rbrace> \<^bold>\<rightarrow> \<lbrace>x\<^sup>T,R\<^sup>T\<rbrace>))] = \<top>" apply simp done
+lemma "[a\<^sup>T \<^bold>=\<^sub>E a\<^sup>T] = \<top>" apply simp nitpick oops -- {* Countermodel by Nitpick *}
 
-lemma "[(a\<^sup>T) \<^bold>=\<^sub>E (a\<^sup>T)] = \<top>" apply simp nitpick oops -- {* Countermodel by Nitpick *}
-
-lemma "[\<lparr>O!,a\<^sup>T\<rparr> \<^bold>\<rightarrow> (a\<^sup>T) \<^bold>=\<^sub>E (a\<^sup>T)] = \<top>" apply simp done
+lemma "[\<lparr>O!,a\<^sup>T\<rparr> \<^bold>\<rightarrow> a\<^sup>T \<^bold>=\<^sub>E a\<^sup>T] = \<top>" apply simp done
 
 lemma "[(\<^bold>\<forall>F. \<lparr>F\<^sup>T,x\<^sup>T\<rparr> \<^bold>\<equiv> \<lparr>F\<^sup>T,x\<^sup>T\<rparr>)] = \<top>" apply simp done
-lemma "[\<lparr>O!,a\<^sup>T\<rparr> \<^bold>\<rightarrow> \<lparr>(\<^bold>\<lambda>x. (x\<^sup>T) \<^bold>=\<^sub>E (a\<^sup>T)),a\<^sup>T\<rparr>] = \<top>" apply simp done
+lemma "[\<lparr>O!,a\<^sup>T\<rparr> \<^bold>\<rightarrow> \<lparr>\<^bold>\<lambda>x. x\<^sup>T \<^bold>=\<^sub>E a\<^sup>T,a\<^sup>T\<rparr>] = \<top>" apply simp done
 
 lemma "[(\<^bold>\<exists>F. \<lbrace>a\<^sup>T,F\<^sup>T\<rbrace>)] = \<top>" apply simp by auto
 
-lemma "[(\<^bold>\<exists>\<phi>. (\<phi>\<^sup>P))] = \<top>" apply simp by auto
-lemma "[(\<^bold>\<exists>\<phi>. (\<phi>\<^sup>F))] = \<top>" apply simp by auto
+lemma "[(\<^bold>\<exists>\<phi>. \<phi>\<^sup>P)] = \<top>" apply simp by auto
+lemma "[(\<^bold>\<exists>\<phi>. \<phi>\<^sup>F)] = \<top>" apply simp by auto
 
 
 section {* Axioms *}
 
 subsection {* Axioms for Negations and Conditionals *}
 
-lemma a21_1_P: "[(\<phi>\<^sup>P) \<^bold>\<rightarrow> ((\<phi>\<^sup>P) \<^bold>\<rightarrow> (\<phi>\<^sup>P))] = \<top>" apply simp done
-lemma a21_1_F: "[(\<phi>\<^sup>F) \<^bold>\<rightarrow> ((\<phi>\<^sup>F) \<^bold>\<rightarrow> (\<phi>\<^sup>F))] = \<top>" apply simp done
-lemma a21_2_P: "[((\<phi>\<^sup>P) \<^bold>\<rightarrow> ((\<psi>\<^sup>P) \<^bold>\<rightarrow> (\<chi>\<^sup>P))) \<^bold>\<rightarrow> (((\<phi>\<^sup>P) \<^bold>\<rightarrow> (\<psi>\<^sup>P)) \<^bold>\<rightarrow> ((\<phi>\<^sup>P) \<^bold>\<rightarrow> (\<chi>\<^sup>P)))] = \<top>" apply simp done
-lemma a21_2_F: "[((\<phi>\<^sup>F) \<^bold>\<rightarrow> ((\<psi>\<^sup>F) \<^bold>\<rightarrow> (\<chi>\<^sup>F))) \<^bold>\<rightarrow> (((\<phi>\<^sup>F) \<^bold>\<rightarrow> (\<psi>\<^sup>F)) \<^bold>\<rightarrow> ((\<phi>\<^sup>F) \<^bold>\<rightarrow> (\<chi>\<^sup>F)))] = \<top>" apply simp done
-lemma a21_3_P: "[(\<^bold>\<not>(\<phi>\<^sup>P) \<^bold>\<rightarrow> \<^bold>\<not>(\<psi>\<^sup>P)) \<^bold>\<rightarrow> ((\<^bold>\<not>(\<phi>\<^sup>P) \<^bold>\<rightarrow> (\<psi>\<^sup>P)) \<^bold>\<rightarrow> (\<phi>\<^sup>P))] = \<top>" apply simp done
-lemma a21_3_F: "[(\<^bold>\<not>(\<phi>\<^sup>F) \<^bold>\<rightarrow> \<^bold>\<not>(\<psi>\<^sup>F)) \<^bold>\<rightarrow> ((\<^bold>\<not>(\<phi>\<^sup>F) \<^bold>\<rightarrow> (\<psi>\<^sup>F)) \<^bold>\<rightarrow> (\<phi>\<^sup>F))] = \<top>" apply simp done
+lemma a21_1_P: "[\<phi>\<^sup>P \<^bold>\<rightarrow> (\<phi>\<^sup>P \<^bold>\<rightarrow> \<phi>\<^sup>P)] = \<top>" apply simp done
+lemma a21_1_F: "[\<phi>\<^sup>F \<^bold>\<rightarrow> (\<phi>\<^sup>F \<^bold>\<rightarrow> \<phi>\<^sup>F)] = \<top>" apply simp done
+lemma a21_2_P: "[(\<phi>\<^sup>P \<^bold>\<rightarrow> (\<psi>\<^sup>P \<^bold>\<rightarrow> \<chi>\<^sup>P)) \<^bold>\<rightarrow> ((\<phi>\<^sup>P \<^bold>\<rightarrow> \<psi>\<^sup>P) \<^bold>\<rightarrow> (\<phi>\<^sup>P \<^bold>\<rightarrow> \<chi>\<^sup>P))] = \<top>" apply simp done
+lemma a21_2_F: "[(\<phi>\<^sup>F \<^bold>\<rightarrow> (\<psi>\<^sup>F \<^bold>\<rightarrow> \<chi>\<^sup>F)) \<^bold>\<rightarrow> ((\<phi>\<^sup>F \<^bold>\<rightarrow> \<psi>\<^sup>F) \<^bold>\<rightarrow> (\<phi>\<^sup>F \<^bold>\<rightarrow> \<chi>\<^sup>F))] = \<top>" apply simp done
+lemma a21_3_P: "[(\<^bold>\<not>\<phi>\<^sup>P \<^bold>\<rightarrow> \<^bold>\<not>\<psi>\<^sup>P) \<^bold>\<rightarrow> ((\<^bold>\<not>\<phi>\<^sup>P \<^bold>\<rightarrow> \<psi>\<^sup>P) \<^bold>\<rightarrow> \<phi>\<^sup>P)] = \<top>" apply simp done
+lemma a21_3_F: "[(\<^bold>\<not>\<phi>\<^sup>F \<^bold>\<rightarrow> \<^bold>\<not>\<psi>\<^sup>F) \<^bold>\<rightarrow> ((\<^bold>\<not>\<phi>\<^sup>F \<^bold>\<rightarrow> \<psi>\<^sup>F) \<^bold>\<rightarrow> \<phi>\<^sup>F)] = \<top>" apply simp done
 
 subsection {* Axioms of Identity *}
 text {* todo *}
@@ -517,26 +535,26 @@ text {* todo *}
 
 subsection {* Axioms of Actuality *}
 
-lemma a31_1_P: "[\<A>(\<^bold>\<not>(\<phi>\<^sup>P)) \<^bold>\<equiv> \<^bold>\<not>(\<A>(\<phi>\<^sup>P))] = \<top>" apply simp done
-lemma a31_1_F: "[\<A>(\<^bold>\<not>(\<phi>\<^sup>F)) \<^bold>\<equiv> \<^bold>\<not>(\<A>(\<phi>\<^sup>F))] = \<top>" apply simp done
-lemma a31_2_P: "[\<A>(\<phi>\<^sup>P \<^bold>\<rightarrow> (\<psi>\<^sup>P)) \<^bold>\<equiv> (\<A>(\<phi>\<^sup>P) \<^bold>\<rightarrow> \<A>(\<psi>\<^sup>P))] = \<top>" apply simp done
-lemma a31_2_F: "[\<A>(\<phi>\<^sup>F \<^bold>\<rightarrow> (\<psi>\<^sup>F)) \<^bold>\<equiv> (\<A>(\<phi>\<^sup>F) \<^bold>\<rightarrow> \<A>(\<psi>\<^sup>F))] = \<top>" apply simp done
-lemma a31_3_P: "[\<A>(\<^bold>\<forall>x. (\<phi>\<^sup>P)) \<^bold>\<equiv> (\<^bold>\<forall>x. \<A>(\<phi>\<^sup>P))] = \<top>" apply simp done
-lemma a31_3_F: "[(\<A>(\<^bold>\<forall>x.(\<phi>\<^sup>F)) \<^bold>\<equiv> (\<^bold>\<forall>x. \<A>(\<phi>\<^sup>F)))] = \<top>" apply simp done
+lemma a31_1_P: "[\<A>(\<^bold>\<not>\<phi>\<^sup>P) \<^bold>\<equiv> \<^bold>\<not>\<A>(\<phi>\<^sup>P)] = \<top>" apply simp done
+lemma a31_1_F: "[\<A>(\<^bold>\<not>\<phi>\<^sup>F) \<^bold>\<equiv> \<^bold>\<not>\<A>(\<phi>\<^sup>F)] = \<top>" apply simp done
+lemma a31_2_P: "[\<A>(\<phi>\<^sup>P \<^bold>\<rightarrow> \<psi>\<^sup>P) \<^bold>\<equiv> (\<A>(\<phi>\<^sup>P) \<^bold>\<rightarrow> \<A>(\<psi>\<^sup>P))] = \<top>" apply simp done
+lemma a31_2_F: "[\<A>(\<phi>\<^sup>F \<^bold>\<rightarrow> \<psi>\<^sup>F) \<^bold>\<equiv> (\<A>(\<phi>\<^sup>F) \<^bold>\<rightarrow> \<A>(\<psi>\<^sup>F))] = \<top>" apply simp done
+lemma a31_3_P: "[\<A>(\<^bold>\<forall>x. \<phi>\<^sup>P) \<^bold>\<equiv> (\<^bold>\<forall>x. \<A>(\<phi>\<^sup>P))] = \<top>" apply simp done
+lemma a31_3_F: "[(\<A>(\<^bold>\<forall>x. \<phi>\<^sup>F) \<^bold>\<equiv> (\<^bold>\<forall>x. \<A>(\<phi>\<^sup>F)))] = \<top>" apply simp done
 lemma a31_4_P: "[\<A>(\<phi>\<^sup>P) \<^bold>\<equiv> \<A>(\<A>(\<phi>\<^sup>P))] = \<top>" apply simp done
 lemma a31_4_F: "[\<A>(\<phi>\<^sup>F) \<^bold>\<equiv> \<A>(\<A>(\<phi>\<^sup>F))] = \<top>" apply simp done
 
 subsection {* Axioms of Necessity *}
 
-lemma a32_1_P: "[(\<^bold>\<box>(\<phi>\<^sup>P \<^bold>\<rightarrow> (\<phi>\<^sup>P))) \<^bold>\<rightarrow> (\<^bold>\<box>(\<phi>\<^sup>P) \<^bold>\<rightarrow> \<^bold>\<box>(\<phi>\<^sup>P))] = \<top>" apply simp done     (* K Schema *)
-lemma a32_1_F: "[(\<^bold>\<box>(\<phi>\<^sup>F \<^bold>\<rightarrow> (\<phi>\<^sup>F))) \<^bold>\<rightarrow> (\<^bold>\<box>(\<phi>\<^sup>F) \<^bold>\<rightarrow> \<^bold>\<box>(\<phi>\<^sup>F))] = \<top>" apply simp done     (* K Schema *)
-lemma a32_2_P: "[\<^bold>\<box>(\<phi>\<^sup>P) \<^bold>\<rightarrow> (\<phi>\<^sup>P)] = \<top>" apply simp done                           (* T Schema *)
-lemma a32_2_F: "[\<^bold>\<box>(\<phi>\<^sup>F) \<^bold>\<rightarrow> (\<phi>\<^sup>F)] = \<top>" apply simp done                           (* T Schema *)
+lemma a32_1_P: "[(\<^bold>\<box>(\<phi>\<^sup>P \<^bold>\<rightarrow> \<phi>\<^sup>P)) \<^bold>\<rightarrow> (\<^bold>\<box>\<phi>\<^sup>P \<^bold>\<rightarrow> \<^bold>\<box>\<phi>\<^sup>P)] = \<top>" apply simp done     (* K Schema *)
+lemma a32_1_F: "[(\<^bold>\<box>(\<phi>\<^sup>F \<^bold>\<rightarrow> \<phi>\<^sup>F)) \<^bold>\<rightarrow> (\<^bold>\<box>\<phi>\<^sup>F \<^bold>\<rightarrow> \<^bold>\<box>\<phi>\<^sup>F)] = \<top>" apply simp done     (* K Schema *)
+lemma a32_2_P: "[\<^bold>\<box>\<phi>\<^sup>P \<^bold>\<rightarrow> \<phi>\<^sup>P] = \<top>" apply simp done                           (* T Schema *)
+lemma a32_2_F: "[\<^bold>\<box>\<phi>\<^sup>F \<^bold>\<rightarrow> \<phi>\<^sup>F] = \<top>" apply simp done                           (* T Schema *)
 
-lemma a32_3_P: "[\<^bold>\<box>(\<^bold>\<diamond>(\<phi>\<^sup>P)) \<^bold>\<rightarrow> \<^bold>\<diamond>(\<phi>\<^sup>P)] = \<top>" apply simp done                       (* 5 Schema *)
-lemma a32_3_F: "[\<^bold>\<box>(\<^bold>\<diamond>(\<phi>\<^sup>F)) \<^bold>\<rightarrow> \<^bold>\<diamond>(\<phi>\<^sup>F)] = \<top>" apply simp done                       (* 5 Schema *)
-lemma a32_4_P: "[(\<^bold>\<forall>x. \<^bold>\<box>(\<phi>\<^sup>P)) \<^bold>\<rightarrow> \<^bold>\<box>((\<^bold>\<forall>x. (\<phi>\<^sup>P)))] = \<top>" apply simp done         (* BF *)
-lemma a32_4_F: "[(\<^bold>\<forall>x. \<^bold>\<box>(\<phi>\<^sup>F)) \<^bold>\<rightarrow> \<^bold>\<box>((\<^bold>\<forall>x. (\<phi>\<^sup>F)))] = \<top>" apply simp done         (* BF *)
+lemma a32_3_P: "[\<^bold>\<box>\<^bold>\<diamond>\<phi>\<^sup>P \<^bold>\<rightarrow> \<^bold>\<diamond>\<phi>\<^sup>P] = \<top>" apply simp done                       (* 5 Schema *)
+lemma a32_3_F: "[\<^bold>\<box>\<^bold>\<diamond>\<phi>\<^sup>F \<^bold>\<rightarrow> \<^bold>\<diamond>\<phi>\<^sup>F] = \<top>" apply simp done                       (* 5 Schema *)
+lemma a32_4_P: "[(\<^bold>\<forall>x. \<^bold>\<box>\<phi>\<^sup>P) \<^bold>\<rightarrow> \<^bold>\<box>((\<^bold>\<forall>x. \<phi>\<^sup>P))] = \<top>" apply simp done         (* BF *)
+lemma a32_4_F: "[(\<^bold>\<forall>x. \<^bold>\<box>\<phi>\<^sup>F) \<^bold>\<rightarrow> \<^bold>\<box>((\<^bold>\<forall>x. \<phi>\<^sup>F))] = \<top>" apply simp done         (* BF *)
 
  text {* The following needs to be an axiom; it does not follow for free: it is possible that there 
 are contingently concrete individuals and it is possible that there are not: *}
@@ -544,13 +562,30 @@ are contingently concrete individuals and it is possible that there are not: *}
 axiomatization where
   a32_5_P: "[\<^bold>\<diamond>(\<^bold>\<exists>x. \<lparr>E\<^sup>T,x\<^sup>T\<rparr> \<^bold>\<and> \<^bold>\<diamond>(\<^bold>\<not>\<lparr>E\<^sup>T,x\<^sup>T\<rparr>)) \<^bold>\<and> \<^bold>\<diamond>(\<^bold>\<not>(\<^bold>\<exists>x. \<lparr>E\<^sup>T,x\<^sup>T\<rparr> \<^bold>\<and> \<^bold>\<diamond>(\<^bold>\<not>\<lparr>E\<^sup>T,x\<^sup>T\<rparr>)))] = \<top>"
 
+  text {* A brief check that this axiom is well-formed, i.e. does not return error *}
+lemma "[\<^bold>\<diamond>(\<^bold>\<exists>x. \<lparr>E\<^sup>T,x\<^sup>T\<rparr> \<^bold>\<and> \<^bold>\<diamond>(\<^bold>\<not>\<lparr>E\<^sup>T,x\<^sup>T\<rparr>)) \<^bold>\<and> \<^bold>\<diamond>(\<^bold>\<not>(\<^bold>\<exists>x. \<lparr>E\<^sup>T,x\<^sup>T\<rparr> \<^bold>\<and> \<^bold>\<diamond>(\<^bold>\<not>\<lparr>E\<^sup>T,x\<^sup>T\<rparr>)))] \<noteq> *" apply simp done
+
 subsection {* Axioms of Necessity and Actuality *}
 
-lemma a33_1_P: "[\<A>(\<phi>\<^sup>P) \<^bold>\<rightarrow> \<^bold>\<box>(\<A>(\<phi>\<^sup>P))] = \<top>" apply simp done
-lemma a33_1_F: "[\<A>(\<phi>\<^sup>F) \<^bold>\<rightarrow> \<^bold>\<box>(\<A>(\<phi>\<^sup>F))] = \<top>" apply simp done
-lemma a33_2_P: "[\<^bold>\<box>(\<phi>\<^sup>P) \<^bold>\<equiv> (\<A>(\<^bold>\<box>(\<phi>\<^sup>P)))] = \<top>" apply simp done
-lemma a33_2_F: "[\<^bold>\<box>(\<phi>\<^sup>F) \<^bold>\<equiv> (\<A>(\<^bold>\<box>(\<phi>\<^sup>F)))] = \<top>" apply simp done
+lemma a33_1_P: "[\<A>(\<phi>\<^sup>P) \<^bold>\<rightarrow> \<^bold>\<box>\<A>(\<phi>\<^sup>P)] = \<top>" apply simp done
+lemma a33_1_F: "[\<A>(\<phi>\<^sup>F) \<^bold>\<rightarrow> \<^bold>\<box>\<A>(\<phi>\<^sup>F)] = \<top>" apply simp done
+lemma a33_2_P: "[\<^bold>\<box>\<phi>\<^sup>P \<^bold>\<equiv> \<A>(\<^bold>\<box>\<phi>\<^sup>P)] = \<top>" apply simp done
+lemma a33_2_F: "[\<^bold>\<box>\<phi>\<^sup>F \<^bold>\<equiv> \<A>(\<^bold>\<box>\<phi>\<^sup>F)] = \<top>" apply simp done
 
+
+subsection {* Axioms for Descriptions *}
+
+ text {* ... here I still run into some problems, need to analyze why both
+ formulas result in errors, check carefully again definition of equality and description ... *}
+
+
+lemma a34_Inst_1: "[(x\<^sup>T \<^bold>= (\<iota> x. \<lparr>R\<^sup>T,x\<^sup>T\<rparr>)) \<^bold>\<equiv> (\<^bold>\<forall> z. (\<A>\<lparr>R\<^sup>T,z\<^sup>T\<rparr> \<^bold>\<equiv> (z\<^sup>T \<^bold>= x\<^sup>T)))] = *" apply simp done
+lemma a34_Inst_2: "[(x\<^sup>T \<^bold>= (\<iota> x. (\<phi>(x))\<^sup>T)) \<^bold>\<equiv> (\<^bold>\<forall> z. (\<A>((\<phi>(z))\<^sup>T) \<^bold>\<equiv> (z\<^sup>T \<^bold>= x\<^sup>T)))] = *" apply simp done
+
+(*
+lemma a34_Inst_test1: "(x\<^sup>T \<^bold>= (\<iota> x. \<lparr>R\<^sup>T,x\<^sup>T\<rparr>)) = X" apply simp oops
+lemma a34_Inst_test2: "(\<^bold>\<forall> z. (\<A>\<lparr>R\<^sup>T,z\<^sup>T\<rparr> \<^bold>\<equiv> (z\<^sup>T \<^bold>= x\<^sup>T))) = X" apply simp oops
+*)
 
 (*<*)
 end
